theories/modules/SModTr.v
@@ -8,27 +8,6 @@ Module SModTr. Section HOARE.
   Context `{!crisG Γ Σ α β τ _S _I}.
   Implicit Types (fn : string) (varg arg : Any.t) (fspo : option fspec_rel) (sp : specmap).
 
-  Definition HoareCall fspo fn varg : itree crisE Any.t :=
-    match fspo with
-    | Some fsp =>
-      PQ <- trigger (Choose (FSpec fsp));;
-
-      (*** precondition ***)
-      arg <- trigger (Choose Any.t);;
-      trigger (Guarantee (PQ.(Precond) varg arg));;;
-
-      (* call *)
-      ret <- trigger (Call fn arg);;
-
-      (*** postcondition ***)
-      vret <- trigger (Take Any.t);;
-      trigger (Assume (PQ.(Postcond) vret ret));;;
-
-      Ret vret
-    | None =>
-        trigger (Call fn varg)
-    end.
-
   Definition HoareFun fspo (body : fbody) : fbody :=
     match fspo with
     | Some fsp =>
@@ -49,14 +28,41 @@ Module SModTr. Section HOARE.
     | None => λ arg, tau;; body arg
     end.
 
+  Definition omask_check (omsk: option emask) fn args : bool :=
+    match omsk with
+    | None => true
+    | Some msk => msk _ (subevent _ (Call fn args))
+    end.
+  
+  Definition HoareCall fspo omsk fn varg : itree crisE Any.t :=
+    match fspo with
+    | Some fsp =>
+      PQ <- trigger (Choose (FSpec (if omask_check omsk fn varg then fsp else fspec_trivial)));;
+
+      (*** precondition ***)
+      arg <- trigger (Choose Any.t);;
+      trigger (Guarantee (PQ.(Precond) varg arg));;;
+
+      (* call *)
+      ret <- trigger (Call fn arg);;
+
+      (*** postcondition ***)
+      vret <- trigger (Take Any.t);;
+      trigger (Assume (PQ.(Postcond) vret ret));;;
+
+      Ret vret
+    | None =>
+        trigger (Call fn varg)
+    end.
+
   (* Wraps a spawn into a Hoare triple *)
   Definition HoareSpawn fspo imgconc fn varg : itree crisE nat :=
     match fspo, imgconc with
     | Some fsp, true =>
-        PQ <- trigger (Choose (FSpec fsp));;
         arg <- trigger (Choose Any.t);;
         tid <- trigger (Spawn fn arg);;
         trigger (Assume (YIELD tid));;;
+        PQ <- trigger (Choose (FSpec fsp));;
         trigger (Guarantee (YIELD tid -∗ TID tid -∗ winv (⊤, ⊤) -∗ (Precond PQ) varg arg));;;
         Ret tid
     | None, true =>
@@ -89,7 +95,7 @@ Module SModTr. Section HOARE.
     else
       trigger GetTid.
 
-  Definition handle sp : crisE ~> itreeV crisE.
+  Definition handle sp (omsk: option emask) : crisE ~> itreeV crisE.
   Proof.
     intros T e.
     destruct e as [e|e].
@@ -97,7 +103,7 @@ Module SModTr. Section HOARE.
     { exact (inr (existT _ (subevent _ e, λ v, Ret v))). }
     destruct e as [[fn args|fn args|tid|]|e].
     (* Call *)
-    { exact (inl (HoareCall (sp.1 !! (fid fn)) fn args)). }
+    { exact (inl (HoareCall (sp.1 !! (fid fn)) omsk fn args)). }
     (* Spawn *)
     { exact (inl (HoareSpawn (sp.1 !! (fid fn)) sp.2 fn args)). }
     (* Yield *)
@@ -108,11 +114,18 @@ Module SModTr. Section HOARE.
     destruct e as [e|e]; exact (inr (existT _ (subevent _ e, λ v, Ret v))).
   Defined.
 
-  Definition trans sp {R} (itr : itree crisE R) : itree crisE R :=
-    interpV (handle sp) itr.
+  Definition _trans sp (omsk: option emask) {R} (itr : itree crisE R) : itree crisE R :=
+    interpV (handle sp omsk) itr.
 
+  Definition trans sp {R} (itr : itree crisE R) : itree crisE R :=
+    _trans sp None itr.
+  
   Definition trans_fnsem (sp : specmap) (sem : option fspec_rel * fbody) : fbody :=
     let '(fspo, fbd) := sem in HoareFun fspo (trans sp ∘ fbd).
+
+  Definition trans_cancel sp (sem : emask * (option fspec_rel * fbody)) : fbody :=
+    let '(msk, (fspo, fbd)) := sem in HoareFun fspo (_trans sp (Some msk) ∘ fbd).
+
 End HOARE. End SModTr.
 
 Global Arguments SModTr.trans_fnsem: simpl never.
@@ -124,60 +137,182 @@ Module SRed. Section RED.
   Import SModTr.
 
   (* reduction lemmas for vis form - used for reduction tactics *)
+
+  Lemma _bind sp omsk (R S : Type) (s : itree crisE R) (k : R → itree crisE S) :
+    _trans sp omsk (s >>= k) = st <- _trans sp omsk s;; _trans sp omsk (k st).
+  Proof using. rewrite /_trans interpV_bind //. Qed.
+
+  Lemma _tau sp omsk (U : Type) (t : itree crisE U) :
+    _trans sp omsk (tau;; t) = tau;; (_trans sp omsk t).
+  Proof using. rewrite /_trans interpV_tau //. Qed.
+
+  Lemma _ret sp omsk (U : Type) (t : U) :
+    _trans sp omsk (Ret t) = Ret t.
+  Proof using. rewrite /_trans interpV_ret //. Qed.
+
+  Lemma _vis_agE sp omsk {X R} (e : agE X) (ktr : X → itree crisE R) :
+    _trans sp omsk (vis e ktr) = vis e (λ x, _trans sp omsk (ktr x)).
+  Proof using.
+    rewrite /_trans /handle /=; apply observe_eta; rewrite /=.
+    f_equal; extensionality x; grind.
+  Qed.
+
+  Lemma _vis_pgE sp omsk  {X R} (e : pgE X) (ktr : X → itree crisE R) :
+    _trans sp omsk  (vis e ktr) = vis e (λ x, _trans sp omsk (ktr x)).
+  Proof using.
+    rewrite /_trans /handle /=; apply observe_eta; rewrite /=.
+    f_equal; extensionality x; grind.
+  Qed.
+
+  Lemma _vis_coreE sp omsk  {X R} (e : coreE X) (ktr : X → itree crisE R) :
+    _trans sp omsk  (vis e ktr) = vis e (λ x, _trans sp omsk (ktr x)).
+  Proof using.
+    rewrite /_trans /handle /=; apply observe_eta; rewrite /=.
+    f_equal; extensionality x; grind.
+  Qed.
+
+  Lemma _vis_call sp omsk {R} fn args (ktr : Any.t → itree crisE R) :
+    _trans sp omsk (vis (Call fn args) ktr) =
+      tau;; r <- HoareCall (sp.1 !! (fid fn)) omsk fn args;;
+      _trans sp omsk (ktr r).
+  Proof using. rewrite /_trans /handle /= interpV_vis. apply observe_eta; ss. Qed.
+
+  Lemma _vis_spawn sp omsk {R} fn args (ktr : nat → itree crisE R) :
+    _trans sp omsk (vis (Spawn fn args) ktr) =
+      tau;; r <- HoareSpawn (sp.1 !! (fid fn)) sp.2 fn args;;
+      _trans sp omsk (ktr r).
+  Proof using. rewrite /_trans /handle /= interpV_vis. apply observe_eta; ss. Qed.
+
+  Lemma _vis_yield sp omsk {R} tid (ktr : () → itree crisE R) :
+    _trans sp omsk (vis (Yield tid) ktr) =
+      tau;; x <- HoareYield sp.2 tid;; _trans sp omsk (ktr x).
+  Proof using. rewrite /_trans /handle /= interpV_vis. apply observe_eta; ss. Qed.
+
+  Lemma _vis_gettid sp omsk {R} (ktr : nat → itree crisE R) :
+    _trans sp omsk (vis GetTid ktr) =
+      tau;; x <- HoareGetTid sp.2;; _trans sp omsk (ktr x).
+  Proof using. rewrite /_trans /handle /= interpV_vis. apply observe_eta; ss. Qed.
+
+  Lemma _assumeK sp omsk {R} P (itr : itree crisE R) :
+    _trans sp omsk (assumeK P itr) = assumeK P (_trans sp omsk itr).
+  Proof using. apply observe_eta; ss; f_equal; extensionality x; grind. Qed.
+
+  Lemma _guaranteeK sp omsk {R} P (itr : itree crisE R) :
+    _trans sp omsk (guaranteeK P itr) = guaranteeK P (_trans sp omsk itr).
+  Proof using. apply observe_eta; ss; f_equal; extensionality x; grind. Qed.
+
+  Lemma _unwrapUK sp omsk {X R} x (ktr : X → itree crisE R) :
+    _trans sp omsk (unwrapUK x ktr) = unwrapUK x (λ x, _trans sp omsk (ktr x)).
+  Proof using. destruct x; ss. eapply observe_eta; ss. f_equal; grind; extensionality x; ss. Qed.
+
+  Lemma _unwrapNK sp omsk {X R} (x : option X) (ktr : X → itree crisE R) :
+    _trans sp omsk (unwrapNK x ktr) = unwrapNK x (λ x, _trans sp omsk (ktr x)).
+  Proof using. destruct x; [des_ifs|]; ss. apply observe_eta; s; f_equal; extensionalities; ss. Qed.
+
+  (* reduction lemmas for trigger form *)
+  Lemma _yield sp omsk tid :
+    _trans sp omsk (trigger (Yield tid)) = tau;; HoareYield sp.2 tid.
+  Proof using. rewrite _vis_yield; grind; erewrite <- bind_ret_r; grind; rewrite _ret //. Qed.
+
+  Lemma _spawn sp omsk fn args :
+    _trans sp omsk (trigger (Spawn fn args)) =
+      tau;; HoareSpawn (sp.1 !! (fid fn)) sp.2 fn args.
+  Proof using. rewrite _vis_spawn; grind; erewrite <- bind_ret_r; grind; rewrite _ret //. Qed.
+
+  Lemma _gettid sp omsk :
+    _trans sp omsk (trigger GetTid) = tau;; HoareGetTid sp.2.
+  Proof using. rewrite _vis_gettid; grind; erewrite <- bind_ret_r; grind; rewrite _ret //. Qed.
+
+  Lemma _call sp omsk fn args :
+    _trans sp omsk (trigger (Call fn args)) =
+    tau;; HoareCall (sp.1 !! (fid fn)) omsk fn args.
+  Proof using. rewrite _vis_call; grind; erewrite <- bind_ret_r; grind; rewrite _ret //. Qed.
+
+  Lemma _pg sp omsk (R : Type) (e : pgE R) : _trans sp omsk (trigger e) = trigger e.
+  Proof using.
+    rewrite _vis_pgE vis_trigger; grind; erewrite <- bind_ret_r; grind; rewrite _ret //.
+  Qed.
+
+  Lemma _core sp omsk (R : Type) (e : coreE R) :
+    _trans sp omsk (trigger e) = trigger e.
+  Proof using.
+    rewrite _vis_coreE vis_trigger; grind; erewrite <- bind_ret_r; grind; rewrite _ret //.
+  Qed.
+
+  Lemma _ag sp omsk (R : Type) (e : agE R) : _trans sp omsk (trigger e) = trigger e.
+  Proof using.
+    rewrite _vis_agE vis_trigger; grind; erewrite <- bind_ret_r; grind; rewrite _ret //.
+  Qed.
+
+  Lemma _ru sp omsk pp : _trans sp omsk (RealUpdate pp) = RealUpdate pp.
+  Proof.
+    rewrite /RealUpdate; unseal CRIS_FancyReal.
+    repeat (rewrite _bind _core; f_equal; extensionalities).
+    repeat (rewrite _bind _ag; f_equal; extensionalities).
+    repeat (rewrite _ag; f_equal; extensionalities).
+  Qed.
+
+  Lemma _ruK {R} sp omsk pp (k : _ → itree _ R) :
+    _trans sp omsk (RealUpdateK pp k) = RealUpdateK pp (λ x, _trans sp omsk (k x)).
+  Proof using. rewrite /RealUpdateK _bind _ru //. Qed.
+
+
+  
+
   Lemma bind sp (R S : Type) (s : itree crisE R) (k : R → itree crisE S) :
     trans sp (s >>= k) = st <- trans sp s;; trans sp (k st).
-  Proof using. rewrite /SModTr.trans interpV_bind //. Qed.
+  Proof using. rewrite /trans /_trans interpV_bind //. Qed.
 
   Lemma tau sp (U : Type) (t : itree crisE U) :
     trans sp (tau;; t) = tau;; (trans sp t).
-  Proof using. rewrite /SModTr.trans interpV_tau //. Qed.
+  Proof using. rewrite /trans /_trans interpV_tau //. Qed.
 
   Lemma ret sp (U : Type) (t : U) :
     trans sp (Ret t) = Ret t.
-  Proof using. rewrite /SModTr.trans interpV_ret //. Qed.
+  Proof using. rewrite /trans /_trans interpV_ret //. Qed.
 
   Lemma vis_agE sp {X R} (e : agE X) (ktr : X → itree crisE R) :
     trans sp (vis e ktr) = vis e (λ x, trans sp (ktr x)).
   Proof using.
-    rewrite /SModTr.trans /SModTr.handle /=; apply observe_eta; rewrite /=.
+    rewrite /trans /_trans /handle /=; apply observe_eta; rewrite /=.
     f_equal; extensionality x; grind.
   Qed.
 
   Lemma vis_pgE sp  {X R} (e : pgE X) (ktr : X → itree crisE R) :
     trans sp  (vis e ktr) = vis e (λ x, trans sp (ktr x)).
   Proof using.
-    rewrite /SModTr.trans /SModTr.handle /=; apply observe_eta; rewrite /=.
+    rewrite /trans /_trans /handle /=; apply observe_eta; rewrite /=.
     f_equal; extensionality x; grind.
   Qed.
 
   Lemma vis_coreE sp  {X R} (e : coreE X) (ktr : X → itree crisE R) :
     trans sp  (vis e ktr) = vis e (λ x, trans sp (ktr x)).
   Proof using.
-    rewrite /SModTr.trans /SModTr.handle /=; apply observe_eta; rewrite /=.
+    rewrite /trans /_trans /handle /=; apply observe_eta; rewrite /=.
     f_equal; extensionality x; grind.
   Qed.
 
   Lemma vis_call sp {R} fn args (ktr : Any.t → itree crisE R) :
     trans sp (vis (Call fn args) ktr) =
-      tau;; r <- HoareCall (sp.1 !! (fid fn)) fn args;;
+      tau;; r <- HoareCall (sp.1 !! (fid fn)) None fn args;;
       trans sp (ktr r).
-  Proof using. rewrite /SModTr.trans /SModTr.handle /= interpV_vis. apply observe_eta; ss. Qed.
+  Proof using. rewrite /trans /_trans /handle /= interpV_vis. apply observe_eta; ss. Qed.
 
   Lemma vis_spawn sp {R} fn args (ktr : nat → itree crisE R) :
     trans sp (vis (Spawn fn args) ktr) =
       tau;; r <- HoareSpawn (sp.1 !! (fid fn)) sp.2 fn args;;
       trans sp (ktr r).
-  Proof using. rewrite /SModTr.trans /SModTr.handle /= interpV_vis. apply observe_eta; ss. Qed.
+  Proof using. rewrite /trans /_trans /handle /= interpV_vis. apply observe_eta; ss. Qed.
 
   Lemma vis_yield sp {R} tid (ktr : () → itree crisE R) :
     trans sp (vis (Yield tid) ktr) =
       tau;; x <- HoareYield sp.2 tid;; trans sp (ktr x).
-  Proof using. rewrite /SModTr.trans /SModTr.handle /= interpV_vis. apply observe_eta; ss. Qed.
+  Proof using. rewrite /trans /_trans /handle /= interpV_vis. apply observe_eta; ss. Qed.
 
   Lemma vis_gettid sp {R} (ktr : nat → itree crisE R) :
     trans sp (vis GetTid ktr) =
       tau;; x <- HoareGetTid sp.2;; trans sp (ktr x).
-  Proof using. rewrite /SModTr.trans /SModTr.handle /= interpV_vis. apply observe_eta; ss. Qed.
+  Proof using. rewrite /trans /_trans /handle /= interpV_vis. apply observe_eta; ss. Qed.
 
   Lemma assumeK sp {R} P (itr : itree crisE R) :
     trans sp (assumeK P itr) = assumeK P (trans sp itr).
@@ -211,7 +346,7 @@ Module SRed. Section RED.
 
   Lemma call sp fn args :
     trans sp (trigger (Call fn args)) =
-    tau;; HoareCall (sp.1 !! (fid fn)) fn args.
+    tau;; HoareCall (sp.1 !! (fid fn)) None fn args.
   Proof using. rewrite vis_call; grind; erewrite <- bind_ret_r; grind; rewrite ret //. Qed.
 
   Lemma pg sp (R : Type) (e : pgE R) : trans sp (trigger e) = trigger e.
@@ -230,7 +365,7 @@ Module SRed. Section RED.
     rewrite vis_agE vis_trigger; grind; erewrite <- bind_ret_r; grind; rewrite ret //.
   Qed.
 
-  Lemma ru sp pp : SModTr.trans sp (RealUpdate pp) = RealUpdate pp.
+  Lemma ru sp pp : trans sp (RealUpdate pp) = RealUpdate pp.
   Proof.
     rewrite /RealUpdate; unseal CRIS_FancyReal.
     repeat (rewrite bind core; f_equal; extensionalities).
@@ -239,6 +374,6 @@ Module SRed. Section RED.
   Qed.
 
   Lemma ruK {R} sp pp (k : _ → itree _ R) :
-    SModTr.trans sp (RealUpdateK pp k) = RealUpdateK pp (λ x, SModTr.trans sp (k x)).
+    trans sp (RealUpdateK pp k) = RealUpdateK pp (λ x, trans sp (k x)).
   Proof using. rewrite /RealUpdateK bind ru //. Qed.
 End RED. End SRed.
